\subsection{Algorithm}

\frame{
    \tableofcontents[ 
        currentsubsection, 
        % hideothersubsections,
        % sectionstyle=show/hide,
        % subsectionstyle=show/shaded,
    ]
}

\begin{frame}{Algorithm}
\begin{algorithm}[H]
    \caption{ADMM} % \label{euclid}
    \begin{algorithmic}[1]
        \Procedure{ADMM}{}\newline
        \textbf{Input:} $y$, $\lambda$, $\rho$, $nb\_iterations$ \\
        \textbf{Output:} $x_{nb\_iterations}$
        \For{\texttt{$k \in 0...nb\_iterations$}}
            \State{$x_{k+1} = \arg\min\limits_{x} {L(x_{k}, z_{k}, u_{k})}$}
            \State{$z_{k+1} = \arg\min\limits_{z} {L(x_{k+1}, z, u_{k})}$}
            \State{$u_{k+1} = u_{k} + \rho (z_{k+1} - x_{k+1})$}
        \EndFor
        \EndProcedure
    \end{algorithmic}
    % \label{alg_1}
\end{algorithm}
\end{frame}

% \begin{frame}{Algorithm General}
% \begin{algorithm}[H]
%     \caption{ADMM} % \label{euclid}
%     \begin{algorithmic}[1]
%         \Procedure{ADMM}{}\newline
%         \textbf{Input:} $g$, $\lambda$, $\rho$, $nb\_iterations$ \\
%         \textbf{Output:} $f_{nb\_iterations}$
%         \For{\texttt{$k \in 0...nb\_iterations$}}
%             \State{$f_{k+1} = \arg\min\limits_{f} {L(f_{k}, z_{k}, u_{k})}$}
%             \State{$z_{k+1} = \arg\min\limits_{z} {L(f_{k+1}, z, u_{k})}$}
%             \State{$u_{k+1} = u_{k} + \rho (z_{k+1} - f_{k+1})$}
%         \EndFor
%         \EndProcedure
%     \end{algorithmic}
%     % \label{alg_1}
% \end{algorithm}
% \end{frame}

% \begin{frame}{$\arg\min\limits_{f} {L(f, z, u)}$}
% \begin{align*}
% &\frac{d}{df} \{
%     \frac{1}{2} \lVert g - Hf \rVert_{2}^{2} 
%     + \lambda R(z) 
%     + \frac{\rho}{2} \lVert f-z+\frac{u}{\rho} \rVert_{2}^{2} 
%     - \frac{\lVert u \rVert_{2}^{2}}{2\rho}
% \} = 0 \\
% &\iff -H^{T} (g - Hf) + \rho (f-z+\frac{u}{\rho}) = 0 \\
% &\iff -H^{T}g + H^{T} H f + \rho f - \rho z + u = 0 \\
% &\iff -H^{T}g + (H^{T}H + \rho I)x - \rho z + u = 0 \\
% &\iff (H^{T}H + \rho I)f = H^{T}y + \rho z - u\\
% &\iff f = (H^{T}H + \rho I)^{-1} (H^{T}g + \rho z - u) \\
% \end{align*}
% \end{frame}

% \begin{frame}{$\arg\min\limits_{z} {L(f, z, u)}$}
% \begin{align*}
% \hat z
% &= \arg\min\limits_{z} L(f, z, u) \\
% &= \arg\min\limits_{z} \{
%     \frac{1}{2} \lVert g - Hf \rVert_{2}^{2} + \lambda R(z) +
%     \frac{\rho}{2} \lVert f-z+\frac{u}{\rho} \rVert_{2}^{2} 
%     - \frac{\lVert u \rVert_{2}^{2}}{2\rho}
% \} \\
% &= \arg\min\limits_{z} \{
%     \lambda R(z) +
%     \frac{\rho}{2} \lVert f-z+\frac{u}{\rho} \rVert_{2}^{2} 
% \} \\
% &= \arg\min\limits_{z} \{
%     \lambda R(z) +
%     \frac{\rho}{2} \lVert z - ( x + \frac{u}{\rho}) \rVert_{2}^{2}
% \} \\
% % &= \arg\min\limits_{z} \{
% %     \lambda R(z) +
% %     \frac{\rho}{2} \lVert -x+z-\frac{u}{\rho} \rVert_{2}^{2} 
% % \}
% \end{align*}
% \end{frame}

% \begin{frame}{Algorithm}
% \begin{algorithm}[H]
% \caption{ADMM} % \label{euclid}
% \begin{algorithmic}[1]
%     \Procedure{ADMM}{}\newline
%     \textbf{Input:} $y$, $\lambda$, $\rho$, $nb\_iterations$ \\
%     \textbf{Output:} $x_{nb\_iterations}$
%     \For{\texttt{$k \in 0...nb\_iterations$}}
%         \State{$f_{k+1} = (H^{T}H + \rho I)^{-1} (\rho z - u - H^{T}g)$}
%         \State{$z_{k+1} = \arg\min\limits_{z} \{
%                 \lambda R(z) +
%                 \frac{\rho}{2} 
%                 \lVert z - ( x + \frac{u}{\rho}) \rVert_{2}^{2}
%             \}$
%         }
%         \State{$u_{k+1} = u_{k} + \rho (z_{k+1} - f_{k+1})$}
%     \EndFor
%     \EndProcedure
% \end{algorithmic}
% % \label{alg_1}
% \end{algorithm}
% \end{frame}